prove total correctness of sum

IMP/coq/ImpVerif.v
@@ -31,6 +31,43 @@ Proof.
     try discriminate; find_inversion; eauto.
 Qed.
 
+Lemma read_write_same :
+  forall h h' a x,
+    write h a x = Some h' ->
+    read h' a = Some x.
+Proof.
+  induction h; simpl; intros.
+  - discriminate.
+  - repeat break_match; repeat find_inversion; auto; try congruence.
+    all: cbn [read]; auto.
+Qed.
+
+Lemma read_write_neq :
+  forall h h' a b x,
+    write h a x = Some h' ->
+    a <> b ->
+    read h' b = read h b.
+Proof.
+  induction h; simpl; intros.
+  - discriminate.
+  - repeat break_match; repeat find_inversion; try congruence.
+    all: cbn[read]; eauto.
+    all: eapply IHh; eauto; omega.
+Qed.
+
+Lemma read_write_nop :
+  forall h a x,
+    read h a = Some x ->
+    write h a x = Some h.
+Proof.
+  induction h; simpl; intros.
+  - discriminate.
+  - destruct a0.
+    + solve_by_inversion.
+    + rewrite IHh; auto.
+    + rewrite IHh; auto.
+Qed.
+
 
 Fixpoint array_at' (base : Z) (contents : list Z) (h : heap) : Prop :=
   match contents with
@@ -69,6 +106,151 @@ Definition array_at (base : Z) (contents : list Z) (h : heap) : Prop :=
   | Some l => l = Vint (Zlength contents) /\
              array_at' (base + 1) contents h
   end.
+
+Lemma array_at_array_at' :
+  forall a l h,
+    array_at a l h ->
+    array_at' (a + 1) l h.
+Proof.
+  unfold array_at.
+  intros.
+  break_match; intuition.
+Qed.
+
+Lemma array_at'_extend_r :
+  forall l h a i x,
+    array_at' a l h ->
+    read h i = Some (Vint x) ->
+    i = a + Zlength l ->
+    array_at' a (l ++ [x]) h.
+Proof.
+  induction l; intros.
+  - rewrite Zlength_correct in *.
+    simpl in *.
+    intuition.
+    assert (i = a) by omega.
+    subst a.
+    auto.
+  - rewrite Zlength_correct in *.
+    simpl in *. intuition.
+    eapply IHl; eauto.
+    zify. omega.
+Qed.
+
+
+Lemma array_at'_extend_l :
+  forall l h a x,
+    array_at' (a + 1) l h ->
+    read h a = Some (Vint x) ->
+    array_at' a (x :: l) h.
+Proof.
+  intros.
+  simpl.
+  intuition.
+Qed.
+
+Lemma array_at'_write_preserve :
+  forall l h h' a i x,
+    array_at' a l h ->
+    write h i x = Some h' ->
+    ~ a <= i < a + Zlength l ->
+    array_at' a l h'.
+Proof.
+  induction l; intros.
+  - simpl. auto.
+  - cbn [array_at'] in *. break_and.
+    rewrite Zlength_correct in *.
+    cbn [Datatypes.length] in *.
+    split.
+    + erewrite read_write_neq; eauto.
+      zify. omega.
+    + eapply IHl; eauto.
+      zify. omega.
+Qed.
+
+Lemma array_at'_write_extend_r :
+  forall l h h' a i x,
+    array_at' a l h ->
+    write h i (Vint x) = Some h' ->
+    i = a + Zlength l ->
+    array_at' a (l ++ [x]) h'.
+Proof.
+  intros.
+  eapply array_at'_extend_r.
+  eapply array_at'_write_preserve.
+  eauto.
+  eauto.
+  omega.
+  erewrite read_write_same; eauto.
+  auto.
+Qed.
+
+
+Lemma array_at'_write_extend_l :
+  forall l h h' a x,
+    array_at' (a + 1) l h ->
+    write h a (Vint x) = Some h' ->
+    array_at' a (x :: l) h'.
+Proof.
+  intros.
+  eapply array_at'_extend_l.
+  eapply array_at'_write_preserve.
+  eauto.
+  eauto.
+  omega.
+  erewrite read_write_same; eauto.
+Qed.
+
+Lemma array_at'_shrink_r :
+  forall l a h,
+    array_at' a l h ->
+    array_at' a (removelast l) h.
+Proof.
+  induction l; simpl; repeat break_match; intuition.
+  cbn [array_at']. intuition.
+Qed.
+
+Lemma array_at'_read_nth :
+  forall contents base h i d,
+    array_at' base contents h ->
+    0 <= i < Zlength contents ->
+    read h (base + i) = Some (Vint (nth (Z.to_nat i) contents d)).
+Proof.
+    induction contents; simpl; intros.
+  - rewrite Zlength_nil in *. omega.
+  - rewrite Zlength_cons in *. break_and.
+    destruct (Z.to_nat i) eqn:?.
+    + simpl. change 0%nat with (Z.to_nat 0) in Heqn.
+      apply Z2Nat.inj in Heqn; try omega.
+      subst i.
+      rewrite Z.add_0_r in *. congruence.
+    + simpl. zify.
+      rewrite Z2Nat.id in * by auto.
+      assert (0 < i) by omega.
+      subst i.
+      replace (base + Z.succ (Z.of_nat n)) with ((base + 1) + Z.of_nat n) by omega.
+      erewrite IHcontents; eauto; try omega.
+      rewrite !Nat2Z.id. eauto.
+Qed.
+
+Lemma array_at'_app :
+  forall l1 a1 a2 l2 h,
+    array_at' a1 l1 h ->
+    array_at' a2 l2 h ->
+    a2 = a1 + Zlength l1 ->
+    array_at' a1 (l1 ++ l2) h.
+Proof.
+  induction l1; simpl; intuition.
+  - rewrite Zlength_nil in *.
+    assert (a2 = a1) by omega.
+    subst a1.
+    auto.
+  - rewrite Zlength_correct in *.
+    cbn [Datatypes.length] in *.
+    eapply IHl1; eauto.
+    zify. omega.
+Qed.
+
 
 Lemma lkup_update :
   forall s x1 x2 v,
@@ -168,4 +350,204 @@ Proof.
   intros.
   break_if; congruence.
 Qed.
+
+Lemma pred_of_dec_false_elim :
+  forall A (B : A -> A -> Prop)
+    (dec : (forall a1 a2 : A, {B a1 a2} + {~ B a1 a2})) a1 a2,
+    pred_of_dec dec a1 a2 = false ->
+    ~ B a1 a2.
+Proof.
+  unfold pred_of_dec.
+  intros.
+  break_if; congruence.
+Qed.
+
+Ltac normalize_Z :=
+      repeat rewrite !Z.add_assoc in *;
+      repeat
+        match goal with
+        | [ H : array_at' ?x _ _ |- _ ] => revert H
+        | [ H : read _ ?x = _  |- _ ] => revert H
+        | [ H : write _ ?x _ = _  |- _ ] => revert H
+        end;
+      repeat (match goal with
+        | [ |- array_at' ?x _ _ -> _ ] => ring_simplify x
+        | [ |- read _ ?x = _ -> _ ] => ring_simplify x
+        | [ |- write _ ?x _ = _ -> _ ] => ring_simplify x
+        end; intro);
+      repeat match goal with
+      | [ |- array_at' ?x _ _ ] => ring_simplify x
+      end;
+      repeat match goal with
+      | [ |- read _ ?x = _ ] => ring_simplify x
+      end;
+      repeat match goal with
+      | [ |- write _ ?x _ = _ ] => ring_simplify x
+      end.
+
+Definition after env s h p (Q : store -> heap -> Prop) : Prop :=
+  exists s' h',
+    eval_s env s h p s' h' /\ Q s' h'.
+
+Lemma after_seq :
+  forall env s h p1 p2 Q,
+    after env s h p1 (fun s' h' => after env s' h' p2 Q) ->
+    after env s h (Sseq p1 p2) Q.
+Proof.
+  unfold after.
+  intros.
+  break_exists.
+  break_and.
+  break_exists.
+  break_and.
+  eauto using eval_seq.
+Qed.
+
+Lemma after_set :
+  forall env s h x e v (Q : store -> heap -> Prop),
+    eval_e s h e v ->
+    Q (update s x v) h ->
+    after env s h (Sset x e) Q.
+Proof.
+  unfold after.
+  intros.
+  eauto using eval_set.
+Qed.
+
+Lemma eval_stmt_while_intro :
+  forall (I : store -> heap -> Prop) (f : store -> nat) env s h e p,
+    I s h ->
+    (forall s0 h0,
+        I s0 h0 ->
+        exists b,
+          eval_e s0 h0 e (Vbool b)) ->
+    (forall s0 h0,
+        I s0 h0 ->
+        eval_e s0 h0 e (Vbool true) ->
+        exists s1 h1,
+          eval_s env s0 h0 p s1 h1 /\
+          I s1 h1 /\
+          (f s1 < f s0)%nat) ->
+    exists s' h',
+      eval_s env s h (Swhile e p) s' h' /\
+      I s' h' /\
+      eval_e s' h' e (Vbool false).
+Proof.
+  intros.
+  assert (forall n s h, (f s < n)%nat -> I s h ->
+                   exists s1 h1,
+                     eval_s env s h (Swhile e p) s1 h1 /\
+                     I s1 h1 /\
+                     eval_e s1 h1 e (Vbool false) /\
+                     (f s1 <= f s)%nat).
+  {
+    induction n; intros.
+    - omega.
+    - copy_apply H0 H3.
+      break_exists.
+      destruct b.
+      + copy_eapply H1 H4; eauto.
+        break_exists. break_and.
+        eapply IHn in H6; [|omega].
+        break_exists_exists.
+        intuition.
+        eauto using eval_while_t.
+      + eauto 10 using eval_while_f.
+  }
+
+  apply H2 with (n := S (f s)) in H; [|omega].
+  break_exists_exists.
+  intuition.
+Qed.
+
+Lemma after_while :
+  forall env s h e p (I Q : store -> heap -> Prop) (f : store -> nat),
+    (forall s0 h0, I s0 h0 -> exists b, eval_e s0 h0 e (Vbool b)) ->
+    I s h ->
+    (forall s0 h0, I s0 h0 -> eval_e s0 h0 e (Vbool true) ->
+              after env s0 h0 p (fun s1 h1 => I s1 h1 /\ (f s1 < f s0)%nat)) ->
+    (forall s0 h0, I s0 h0 -> eval_e s0 h0 e (Vbool false) -> Q s0 h0) ->
+    after env s h (Swhile e p) Q.
+Proof.
+  unfold after.
+  intros.
+  pose proof eval_stmt_while_intro I f env s h e p.
+  repeat concludes.
+  firstorder.
+Qed.
+
+Lemma nth_error_nth :
+  forall A (l : list A) n x d,
+    nth_error l n = Some x ->
+    nth n l d = x.
+Proof.
+  induction l; destruct n; simpl; intros; try discriminate.
+  - congruence.
+  - eauto.
+Qed.
+
+Lemma nth_nth_error :
+  forall A (l : list A) n d,
+    (0 <= n < Datatypes.length l)%nat ->
+    nth_error l n = Some (nth n l d).
+Proof.
+  induction l; destruct n; simpl; intros.
+  - omega.
+  - omega.
+  - auto.
+  - apply IHl. omega.
+Qed.
+
+Lemma array_at'_nth_error_read :
+  forall contents base h x i,
+    array_at' base contents h ->
+    0 <= i < Zlength contents ->
+    nth_error contents (Z.to_nat i) = Some x ->
+    read h (base + i) = Some (Vint x).
+Proof.
+  induction contents; simpl; intros.
+  - rewrite Zlength_nil in *. omega.
+  - break_and.
+    generalize dependent i.
+    refine (natlike_ind _ _ _); intros.
+    + simpl in *. find_inversion. rewrite Z.add_0_r. auto.
+    + rewrite Z2Nat.inj_succ in * by auto.
+      simpl in *.
+      rewrite <- Z.add_succ_comm.
+      apply IHcontents; auto.
+      rewrite Zlength_cons in *. omega.
+Qed.
+
+Lemma array_at'_nth_read :
+  forall contents base h i,
+    array_at' base contents h ->
+    0 <= i < Zlength contents ->
+    read h (base + i) = Some (Vint (nth (Z.to_nat i) contents 0)).
+Proof.
+  intros.
+  assert (exists x, nth_error contents (Z.to_nat i) = Some x).
+  {
+    destruct (nth_error contents (Z.to_nat i)) eqn:?; eauto.
+    exfalso.
+    find_apply_lem_hyp nth_error_None.
+    rewrite Zlength_correct in *.
+    zify. rewrite Z2Nat.id in * by omega. omega. }
+  break_exists.
+  eapply array_at'_nth_error_read; eauto.
+  erewrite nth_error_nth; eauto.
+Qed.
+
+Lemma array_at_read_nth :
+  forall contents base h i,
+    array_at base contents h ->
+    0 <= i < Zlength contents ->
+    read h (Z.succ (base + i)) = Some (Vint (nth (Z.to_nat i) contents 0)).
+Proof.
+  intros.
+  rewrite <- Z.add_succ_l.
+  eapply array_at'_nth_read.
+  eauto using array_at_array_at'.
+  auto.
+Qed.
+
 
